TM/Basic/WriteString.v
@@ -1,4 +1,5 @@
 Require Import TM.TM TM.Basic.Mono TM.Combinators.SequentialComposition.
+Require Import List.
 
 Section Write_String.
 
